src/LibListSub.v
@@ -1,3 +1,5 @@
+(*--- under construction
+
 (**************************************************************************
 * TLC: A library for Coq                                                  *
 * Sub-lists                                                               *
@@ -325,3 +327,5 @@ Qed.
 End PrefixClosed.
 
 
+
+*)
